SmallStep.v
@@ -16,6 +16,36 @@ Module SmallStep.
 Import Ir.Inst.
 
 
+Definition pc_bbid (p:Ir.IRFunction.pc): nat :=
+  match p with
+  | Ir.IRFunction.pc_phi bbid _ => bbid
+  | Ir.IRFunction.pc_inst bbid _ => bbid
+  | Ir.IRFunction.pc_terminator bbid => bbid
+  end.
+
+Definition incrpc (c:Ir.Config.t) :=
+  match (Ir.Config.s c) with
+  | (cid, pc0)::t =>
+    match Ir.Config.get_funid c cid with
+    | Some funid =>
+      match (Ir.IRModule.getf funid (Ir.Config.md c)) with
+      | None => c (* Cannot happen *)
+      | Some fdef =>
+        match (Ir.IRFunction.next_trivial_pc pc0 fdef) with
+        | Some pc' =>
+          Ir.Config.update_pc c pc'
+        | None => c (* Cannot happen..! *)
+        end
+      end
+    | None => c (* Cannot happen *)
+    end
+  | nil => c (* Cannot happen *)
+  end.
+
+Definition update_reg_and_incrpc (c:Ir.Config.t) (r:Ir.reg) (v:Ir.val) :=
+  incrpc (Ir.Config.update_rval c r v).
+
+
 Definition twos_compl (n:N) (sz:nat):N :=
   N.modulo n (N.shiftl 2%N (N.of_nat sz)).
 
@@ -56,20 +86,34 @@ Definition psub p1 p2 m bsz :=
     Ir.num (twos_compl_sub (N.of_nat o1) (N.of_nat o2) bsz)
   end.
 
-Definition gep (p:Ir.ptrval) (idx:N) (t:Ir.ty) (m:Ir.Memory.t): Ir.val :=
+Definition gep (p:Ir.ptrval) (idx0:N) (t:Ir.ty) (m:Ir.Memory.t) (inb:bool): Ir.val :=
+  let idx := N.mul idx0 (N.of_nat (Ir.ty_bytesz t)) in
   match p with
   | Ir.plog (l, o) =>
-    match (Ir.Memory.get m l) with
-    | Some blk =>
-      let o' := (N.to_nat (twos_compl_add (N.of_nat o) idx Ir.PTRSZ)) in
-      if Ir.MemBlock.inbounds o blk &&
-         Ir.MemBlock.inbounds o' blk then Ir.ptr (Ir.plog (l, o'))
-      else Ir.poison (* out of bounds *)
-    | None => Ir.poison (* unreachable *)
-    end
+    let o' := N.to_nat (twos_compl_add (N.of_nat o) idx Ir.PTRSZ) in
+    if inb then
+      match (Ir.Memory.get m l) with
+      | Some blk =>
+        if Ir.MemBlock.inbounds o blk &&
+           Ir.MemBlock.inbounds o' blk then Ir.ptr (Ir.plog (l, o'))
+        else Ir.poison (* out of bounds *)
+      | None => Ir.poison (* unreachable *)
+      end
+    else Ir.ptr (Ir.plog (l, o'))
   | Ir.pphy (o, Is, cid) =>
-    Ir.ptr (Ir.pphy (o,
-                     (N.to_nat (twos_compl_add (N.of_nat o) idx Ir.PTRSZ))::Is, cid))
+    let o' := N.to_nat (twos_compl_add (N.of_nat o) idx Ir.PTRSZ) in
+    if inb then
+      if N.ltb idx (N.shiftl 1 (N.sub (N.of_nat Ir.PTRSZ) 1%N)) then
+        (* Added idx is positive. *)
+        if Nat.ltb o' Ir.MEMSZ then
+          (* Should not overflow Ir.MEMSZ *)
+          Ir.ptr (Ir.pphy (o', o::o'::Is, cid))
+        else Ir.poison
+      else
+        (* idx is negative: no constraint. *)
+        Ir.ptr (Ir.pphy (o', o::o'::Is, cid))
+    else
+      Ir.ptr (Ir.pphy (o', Is, cid))
   end.
 
 Definition free p m: option (Ir.Memory.t) :=
@@ -89,13 +133,54 @@ Definition free p m: option (Ir.Memory.t) :=
 Definition to_num (b:bool): Ir.val :=
   Ir.num (if b then 1%N else 0%N).
 
+Definition icmp_eq_ptr (p1 p2:Ir.ptrval) (m:Ir.Memory.t): option bool :=
+  match (p1, p2) with
+  | (Ir.plog (l1, o1), Ir.plog (l2, o2)) =>
+    if Nat.eqb l1 l2 then
+      (* ICMP-PTR-LOGICAL *)
+      Some (Nat.eqb o1 o2)
+    else
+      match (Ir.Memory.get m l1, Ir.Memory.get m l2) with
+      | (Some mb1, Some mb2) =>
+        (* ICMP-PTR-LOGICAL' *)
+        if Nat.leb o1 (Ir.MemBlock.n mb1) && Nat.leb o2 (Ir.MemBlock.n mb2) then
+          Some false
+        else
+          (* ICMP-PTR-LOGICAL-NONDET-TRUE *)
+          None
+      | (_, _) => None
+      end
+  | (Ir.pphy (o1, Is1, cid1), _) =>
+    Some (N.eqb (N.of_nat o1) (p2N p2 m Ir.PTRSZ))
+  | (_, Ir.pphy (o2, Is2, cid2)) =>
+    Some (N.eqb (p2N p1 m Ir.PTRSZ) (N.of_nat o2))
+  end.
+
+Definition icmp_ule_ptr (p1 p2:Ir.ptrval) (m:Ir.Memory.t): option bool :=
+  match (p1, p2) with
+  | (Ir.plog (l1, o1), Ir.plog (l2, o2)) =>
+    if Nat.eqb l1 l2 then
+      match (Ir.Memory.get m l1, Ir.Memory.get m l2) with
+      | (Some mb1, Some mb2) =>
+        if Nat.leb o1 (Ir.MemBlock.n mb1) && Nat.leb o2 (Ir.MemBlock.n mb2) then
+          Some (Nat.leb o1 o2)
+        else None (* nondet. value *)
+      | (_, _) => None
+      end
+    else None (* nondet. value *)
+  | (Ir.pphy (o1, Is1, cid1), _) =>
+    Some (N.leb (N.of_nat o1) (p2N p2 m Ir.PTRSZ))
+  | (_, Ir.pphy (o2, Is2, cid2)) =>
+    Some (N.leb (p2N p1 m Ir.PTRSZ) (N.of_nat o2))
+  end.
+
 (* Semantics of instructions which behave deterministically. *)
-Definition step_det (c:Ir.Config.t) (i:Ir.Inst.t)
+Definition inst_det (c:Ir.Config.t) (i:Ir.Inst.t)
 : option (Ir.event * Ir.Config.t) :=
   match i with
   | iadd r (Ir.ity bsz) op1 op2 =>
     Some (Ir.e_none,
-      Ir.Config.update_rval c r
+      update_reg_and_incrpc c r
       match (Ir.Config.get_val c op1, Ir.Config.get_val c op2) with
       | (Some (Ir.num i1), Some (Ir.num i2)) =>
         Ir.num (twos_compl_add i1 i2 bsz)
@@ -104,7 +189,7 @@ Definition step_det (c:Ir.Config.t) (i:Ir.Inst.t)
 
   | isub r (Ir.ity bsz) op1 op2 =>
     Some (Ir.e_none,
-      Ir.Config.update_rval c r
+      update_reg_and_incrpc c r
       match (Ir.Config.get_val c op1, Ir.Config.get_val c op2) with
       | (Some (Ir.num i1), Some (Ir.num i2)) =>
         Ir.num (twos_compl_sub i1 i2 bsz)
@@ -113,7 +198,7 @@ Definition step_det (c:Ir.Config.t) (i:Ir.Inst.t)
 
   | ipsub r (Ir.ity bsz) (Ir.ptrty opty) op1 op2 =>
     Some (Ir.e_none,
-      Ir.Config.update_rval c r
+      update_reg_and_incrpc c r
       match (Ir.Config.get_val c op1, Ir.Config.get_val c op2) with
       | (Some (Ir.ptr p1), Some (Ir.ptr p2)) =>
         psub p1 p2 (Ir.Config.m c) bsz
@@ -122,10 +207,10 @@ Definition step_det (c:Ir.Config.t) (i:Ir.Inst.t)
 
   | igep r (Ir.ptrty retty) opptr opidx inb =>
     Some (Ir.e_none,
-      Ir.Config.update_rval c r
+      update_reg_and_incrpc c r
       match (Ir.Config.get_val c opptr, Ir.Config.get_val c opidx) with
       | (Some (Ir.ptr p), Some (Ir.num idx)) =>
-        gep p idx retty (Ir.Config.m c)
+        gep p idx retty (Ir.Config.m c) inb
       | (_, _) => Ir.poison
       end)
 
@@ -134,7 +219,7 @@ Definition step_det (c:Ir.Config.t) (i:Ir.Inst.t)
     | (Some (Ir.ptr p)) =>
       if Ir.deref (Ir.Config.m c) p (Ir.ty_bytesz retty) then
         Some (Ir.e_none,
-              (Ir.Config.update_rval c r
+              (update_reg_and_incrpc c r
               (Ir.load_val (Ir.Config.m c) p retty)))
       else None
     | _ => None
@@ -145,7 +230,7 @@ Definition step_det (c:Ir.Config.t) (i:Ir.Inst.t)
     | (Some (Ir.ptr p), Some v) =>
       if Ir.deref (Ir.Config.m c) p (Ir.ty_bytesz valty) then
         Some (Ir.e_none,
-              Ir.Config.update_m c (Ir.store_val (Ir.Config.m c) p v valty))
+              incrpc (Ir.Config.update_m c (Ir.store_val (Ir.Config.m c) p v valty)))
       else None
     | (_, _) => None
     end
@@ -158,21 +243,21 @@ Definition step_det (c:Ir.Config.t) (i:Ir.Inst.t)
     match (Ir.Config.get_val c opptr) with
     | Some (Ir.ptr p) =>
       match (free p (Ir.Config.m c)) with
-      | Some m => Some (Ir.e_none, Ir.Config.update_m c m)
+      | Some m => Some (Ir.e_none, incrpc (Ir.Config.update_m c m))
       | None => None
       end
     | _ => None
     end
 
   | iptrtoint r opptr (Ir.ity retty) =>
-    Some (Ir.e_none, Ir.Config.update_rval c r
+    Some (Ir.e_none, update_reg_and_incrpc c r
       match (Ir.Config.get_val c opptr) with
       | Some (Ir.ptr p) => (Ir.num (p2N p (Ir.Config.m c) retty))
       | _ => Ir.poison
       end)
 
   | iinttoptr r opint (Ir.ptrty retty) =>
-    Some (Ir.e_none, Ir.Config.update_rval c r
+    Some (Ir.e_none, update_reg_and_incrpc c r
       match (Ir.Config.get_val c opint) with
       | Some (Ir.num n) =>
         Ir.ptr (Ir.pphy (N.to_nat n, nil, None))
@@ -181,7 +266,7 @@ Definition step_det (c:Ir.Config.t) (i:Ir.Inst.t)
 
   | ievent opval =>
     match (Ir.Config.get_val c opval) with
-    | Some v => Some (Ir.e_some v, c)
+    | Some v => Some (Ir.e_some v, incrpc c)
     | None => None
     end
 
@@ -189,49 +274,56 @@ Definition step_det (c:Ir.Config.t) (i:Ir.Inst.t)
     match (Ir.Config.get_val c op1, Ir.Config.get_val c op2) with
     (* Integer comparison *)
     | (Some (Ir.num n1), Some (Ir.num n2)) =>
-      Some (Ir.e_none, Ir.Config.update_rval c r (to_num (N.eqb n1 n2)))
+      Some (Ir.e_none, update_reg_and_incrpc c r (to_num (N.eqb n1 n2)))
     (* Comparison with poison *)
     | (Some (Ir.poison), _) =>
-      Some (Ir.e_none, Ir.Config.update_rval c r Ir.poison)
+      Some (Ir.e_none, update_reg_and_incrpc c r Ir.poison)
     | (_, Some (Ir.poison)) =>
-      Some (Ir.e_none, Ir.Config.update_rval c r Ir.poison)
+      Some (Ir.e_none, update_reg_and_incrpc c r Ir.poison)
     (* Pointer comparison *)
     | (Some (Ir.ptr p1), Some (Ir.ptr p2)) =>
-      let m := Ir.Config.m c in
-      match (p1, p2) with
-      | (Ir.plog (l1, o1), Ir.plog (l2, o2)) =>
-        if Nat.eqb l1 l2 then
-          (* ICMP-PTR-LOGICAL *)
-          Some (Ir.e_none, Ir.Config.update_rval c r (to_num (Nat.eqb o1 o2)))
-        else
-          match (Ir.Memory.get m l1, Ir.Memory.get m l2) with
-          | (Some mb1, Some mb2) =>
-            (* ICMP-PTR-LOGICAL' *)
-            if Nat.leb o1 (Ir.MemBlock.n mb1) && Nat.leb o2 (Ir.MemBlock.n mb2) then
-              Some (Ir.e_none, Ir.Config.update_rval c r (to_num false))
-            else
-              (* ICMP-PTR-LOGICAL-NONDET-TRUE *)
-              None
-          | (_, _) => None
-          end
-      | (Ir.pphy (o1, Is1, cid1), _) =>
-        Some (Ir.e_none, Ir.Config.update_rval c r
-               (to_num (N.eqb (N.of_nat o1) (p2N p2 m Ir.PTRSZ))))
-      | (_, Ir.pphy (o2, Is2, cid2)) =>
-        Some (Ir.e_none, Ir.Config.update_rval c r
-               (to_num (N.eqb (p2N p1 m Ir.PTRSZ) (N.of_nat o2))))
+      match (icmp_eq_ptr p1 p2 (Ir.Config.m c)) with
+      | Some b => Some (Ir.e_none, update_reg_and_incrpc c r (to_num b))
+      | None => None
       end
-    | (_, _) => None (* In other cases, it is nondeterministic. *)
+    | (_, _) => None (* In other cases, it is untyped. *)
     end
 
-  | iicmp_ule r opty opptr1 opttr2 =>
+  | iicmp_ule r opty opptr1 opptr2 =>
     match (Ir.Config.get_val c opptr1, Ir.Config.get_val c opptr2) with
+    (* Integer comparison *)
     | (Some (Ir.num n1), Some (Ir.num n2)) =>
-      Nat.leb n1 n2
-    |
+      Some (Ir.e_none, update_reg_and_incrpc c r (to_num (N.leb n1 n2)))
+    (* Comparison with poison *)
+    | (Some Ir.poison, _) =>
+      Some (Ir.e_none, update_reg_and_incrpc c r Ir.poison)
+    | (_, Some Ir.poison) =>
+      Some (Ir.e_none, update_reg_and_incrpc c r Ir.poison)
+    (* Comparison with pointer *)
+    | (Some (Ir.ptr p1), Some (Ir.ptr p2)) =>
+      match (icmp_ule_ptr p1 p2 (Ir.Config.m c)) with
+      | Some b => Some (Ir.e_none, update_reg_and_incrpc c r (to_num b))
+      | None => None
+      end
+    | (_, _) => None
+    end
 
   | _ => None (* Untyped IR *)
   end.
+
+
+
+(* Semantics of terminators. *)
+Definition t_step (c:Ir.Config.t) (t:Ir.Terminator.t): option Ir.Config.t :=
+  match t with
+  | Ir.Terminator.tbr bbid => .. (* get_begin_pc_bb bbid fdef *)
+  | Ir.Terminator.tbr_cond condop bbid1 bbid2 => ..
+  | Ir.Terminator.tret retop => ..
+  end.
+
+(* Semantics of phi nodes. *)
+Definition phi_step (c:Ir.Config.t) (p:Ir.PhiNode.t): option Ir.Config.t :=
+  ..
 
 End SmallStep.
 
